Lean4Lean/Verify/NameGenerator.lean
@@ -3,8 +3,8 @@ import Lean4Lean.Theory.VExpr
 
 namespace Lean.NameGenerator
 
-def Reserves (ngen : NameGenerator) (fvars : List FVarId) : Prop :=
-  ∀ fv ∈ fvars, ∀ i, fv = ⟨.num ngen.namePrefix i⟩ → i < ngen.idx
+def Reserves (ngen : NameGenerator) (fv : FVarId) : Prop :=
+  ∀ i, fv = ⟨.num ngen.namePrefix i⟩ → i < ngen.idx
 
 protected inductive LE : NameGenerator → NameGenerator → Prop where
   | le : i ≤ j → NameGenerator.LE ⟨pfx, i⟩ ⟨pfx, j⟩
@@ -16,5 +16,5 @@ theorem LE.rfl {ngen : NameGenerator} : ngen ≤ ngen := ⟨Nat.le_refl _⟩
 theorem LE.trans {ngen₁ ngen₃ ngen₃ : NameGenerator} : ngen₁ ≤ ngen₂ → ngen₂ ≤ ngen₃ → ngen₁ ≤ ngen₃
   | ⟨h₁⟩, ⟨h₂⟩ => ⟨Nat.le_trans h₁ h₂⟩
 
-theorem Reserves.mono : ngen ≤ ngen' → fvars' ⊆ fvars → Reserves ngen fvars → Reserves ngen' fvars'
-  | ⟨h₁⟩, h₂ => fun H _ hfv _ hi => Nat.lt_of_lt_of_le (H _ (h₂ hfv) _ hi) h₁
+theorem Reserves.mono : ngen ≤ ngen' → Reserves ngen fv → Reserves ngen' fv
+  | ⟨h₁⟩ => fun H _ hi => Nat.lt_of_lt_of_le (H _ hi) h₁
